src/riot/RIoT.X509.DeviceIDCRI.Attributes.fsti
@@ -48,7 +48,12 @@ open LowParse.Spec.Bytes
  *   }
  *)
 
-#set-options "--z3rlimit 128 --fuel 0 --ifuel 0"
+#set-options "--z3rlimit 128 --fuel 0 --ifuel 0 --using_facts_from '* -FStar.Tactics -FStar.Reflection'"
+
+#set-options "--__temp_no_proj RIoT.X509.DeviceIDCRI.Attributes"
+
+val decl : unit
+
 type deviceIDCRI_attributes_extensionRequest_payload_t = {
   deviceID_attr_ext_key_usage: key_usage_t
 }
