src/riot/RIoT.X509.DeviceIDCRI.Subject.fsti
@@ -13,6 +13,8 @@ module B32 = FStar.Bytes
 
 #set-options "--__temp_no_proj RIoT.X509.DeviceIDCRI.Subject"
 
+val decl : unit
+
 noeq
 type deviceIDCRI_subject_payload_t = {
   deviceIDCRI_subject_Common      : x509_RDN_x520_attribute_t COMMON_NAME  IA5_STRING;
